Rename fmap_add to fun_merge

Launchbury/Env.thy
@@ -129,43 +129,43 @@ lemma fmap_restr_fmap_delete_other[simp]: "x \<notin> S \<Longrightarrow> fmap_d
 lemma fmap_delete_restr: "fmap_delete x m = m f|` (-{x})"
   by (auto simp add: lookup_fmap_restr_eq)
 
-subsubsection {* Addition (merging) of finite maps *}
+subsubsection {* Merging of two functions *}
 
-definition fmap_add :: "'a set \<Rightarrow> ('a \<Rightarrow> 'b) \<Rightarrow> ('a \<Rightarrow> 'b) \<Rightarrow> ('a \<Rightarrow> 'b)"
-  where "fmap_add S f1 f2 = (\<lambda> x. if x \<in> S then f2 x else f1 x)"
+definition fun_merge :: "'a set \<Rightarrow> ('a \<Rightarrow> 'b) \<Rightarrow> ('a \<Rightarrow> 'b) \<Rightarrow> ('a \<Rightarrow> 'b)"
+  where "fun_merge S f1 f2 = (\<lambda> x. if x \<in> S then f2 x else f1 x)"
 
-abbreviation fmap_add_syn ("_ f++\<^bsub>_\<^esub> _" [100, 0, 100] 100) where "f1 f++\<^bsub>S\<^esub> f2 \<equiv> fmap_add S f1 f2"
+abbreviation fun_merge_syn ("_ f++\<^bsub>_\<^esub> _" [100, 0, 100] 100) where "f1 f++\<^bsub>S\<^esub> f2 \<equiv> fun_merge S f1 f2"
 
-lemma fmap_add_fempty[simp]: "\<bottom> f++\<^bsub>S\<^esub> m = m f|` S" 
-  by (auto simp add: fmap_add_def fmap_restr_def)
+lemma fun_merge_fempty[simp]: "\<bottom> f++\<^bsub>S\<^esub> m = m f|` S" 
+  by (auto simp add: fun_merge_def fmap_restr_def)
 
-lemma fmap_add_fempty2[simp]: "m f++\<^bsub>S\<^esub> \<bottom> = m f|` (-S)" 
-  by (auto simp add: fmap_add_def fmap_restr_def)
+lemma fun_merge_fempty2[simp]: "m f++\<^bsub>S\<^esub> \<bottom> = m f|` (-S)" 
+  by (auto simp add: fun_merge_def fmap_restr_def)
 
-lemma fdom_fmap_add[simp]: "fdom (m1 f++\<^bsub>S\<^esub> m2) = (fdom m1 - S) \<union> (fdom m2 \<inter> S)"
-  by (auto simp add: fmap_add_def fdom_def)
+lemma fdom_fun_merge[simp]: "fdom (m1 f++\<^bsub>S\<^esub> m2) = (fdom m1 - S) \<union> (fdom m2 \<inter> S)"
+  by (auto simp add: fun_merge_def fdom_def)
 
-lemma lookup_fmap_add1[simp]: "x \<in> S \<Longrightarrow> (m1 f++\<^bsub>S\<^esub> m2) x = m2 x"
-  by (auto simp add: fmap_add_def fdom_def)
+lemma lookup_fun_merge1[simp]: "x \<in> S \<Longrightarrow> (m1 f++\<^bsub>S\<^esub> m2) x = m2 x"
+  by (auto simp add: fun_merge_def fdom_def)
 
-lemma lookup_fmap_add2[simp]:  "x \<notin> S \<Longrightarrow> (m1 f++\<^bsub>S\<^esub> m2) x = m1 x"
-  by (auto simp add: fmap_add_def fdom_def)
+lemma lookup_fun_merge2[simp]:  "x \<notin> S \<Longrightarrow> (m1 f++\<^bsub>S\<^esub> m2) x = m1 x"
+  by (auto simp add: fun_merge_def fdom_def)
 
-lemma lookup_fmap_add_eq: "(m1 f++\<^bsub>S\<^esub> m2) x = (if x \<in> S then m2 x else m1 x)"
+lemma lookup_fun_merge_eq: "(m1 f++\<^bsub>S\<^esub> m2) x = (if x \<in> S then m2 x else m1 x)"
   by (cases "x \<notin> S") simp_all
 
-lemma fmap_add_upd_swap: 
+lemma fun_merge_upd_swap: 
   "x \<notin> S \<Longrightarrow> \<rho>(x := z) f++\<^bsub>S\<^esub> \<rho>' = (\<rho> f++\<^bsub>S\<^esub> \<rho>')(x := z)"
-  by (auto simp add: fmap_add_def  fdom_def)
+  by (auto simp add: fun_merge_def  fdom_def)
 
-lemma fmap_add_upd: 
+lemma fun_merge_upd: 
   "x \<in> S \<Longrightarrow> \<rho> f++\<^bsub>S\<^esub> (\<rho>'(x := z)) = (\<rho> f++\<^bsub>S - {x}\<^esub> \<rho>')(x := z)"
-  by (auto simp add: fmap_add_def  fdom_def)
+  by (auto simp add: fun_merge_def  fdom_def)
 
-lemma fmap_restr_add: "fmap_restr S (m1 f++\<^bsub>S2\<^esub> m2) = fmap_restr S m1 f++\<^bsub>S2\<^esub> fmap_restr S m2"
-  by (auto simp add: fmap_add_def  fdom_def fmap_restr_def)
+lemma fmap_restr_add: "(m1 f++\<^bsub>S2\<^esub> m2) f|` S = m1 f|` S f++\<^bsub>S2\<^esub> m2 f|` S"
+  by (auto simp add: fun_merge_def  fdom_def fmap_restr_def)
 
 lemma fmap_delete_add: "fmap_delete x (m1 f++\<^bsub>S\<^esub> m2) = fmap_delete x m1 f++\<^bsub>S - {x}\<^esub> fmap_delete x m2"
-  by (auto simp add: fmap_add_def  fdom_def fmap_restr_def fmap_delete_def)
+  by (auto simp add: fun_merge_def  fdom_def fmap_restr_def fmap_delete_def)
 
 end
